added yield invariant

Test/civl/treiber-stack2.bpl
@@ -86,6 +86,10 @@ modifies ts;
 procedure {:yields} {:layer 0} {:refines "AtomicWriteTopOfStack"} 
 WriteTopOfStack(ref_t: RefTreiber X, old_ref_n: RefNode X, new_ref_n: RefNode X) returns (r: bool);
 
+procedure {:yield_invariant} {:layer 2} YieldInv(ref_t: RefTreiber X);
+requires ts->dom[ref_t];
+requires BetweenSet(ts->val[ref_t]->stack->val, ts->val[ref_t]->top, Nil())[ts->val[ref_t]->top];
+requires Subset(BetweenSet(ts->val[ref_t]->stack->val, ts->val[ref_t]->top, Nil()), Union(Singleton(Nil()), ts->val[ref_t]->stack->dom));
 
 // Contents of node.bpl
 
@@ -94,53 +98,53 @@ type RefNode T = Ref (Node T);
 function Nil<T>(): RefNode T;
 function {:constructor} Node<T>(next: RefNode T, val: T): Node T;
 
-function Between<T>(f: [RefNode T]RefNode T, x: RefNode T, y: RefNode T, z: RefNode T): bool;
-function Avoiding<T>(f: [RefNode T]RefNode T, x: RefNode T, y: RefNode T, z: RefNode T): bool;
-function {:inline} BetweenSet<T>(f:[RefNode T]RefNode T, x: RefNode T, z: RefNode T): [RefNode T]bool
+function Between<T>(f: [RefNode T]Node T, x: RefNode T, y: RefNode T, z: RefNode T): bool;
+function Avoiding<T>(f: [RefNode T]Node T, x: RefNode T, y: RefNode T, z: RefNode T): bool;
+function {:inline} BetweenSet<T>(f:[RefNode T]Node T, x: RefNode T, z: RefNode T): [RefNode T]bool
 {
   (lambda y: RefNode T :: Between(f, x, y, z))
 }
 
 // reflexive
-axiom {:ctor "Node"} (forall<T> f: [RefNode T]RefNode T, x: RefNode T :: Between(f, x, x, x));
+axiom {:ctor "Node"} (forall<T> f: [RefNode T]Node T, x: RefNode T :: Between(f, x, x, x));
 
 // step
-axiom {:ctor "Node"} (forall<T> f: [RefNode T]RefNode T, x: RefNode T, y: RefNode T, z: RefNode T, w: RefNode T :: {Between(f, y, z, w), f[x]} Between(f, x, f[x], f[x]));
+axiom {:ctor "Node"} (forall<T> f: [RefNode T]Node T, x: RefNode T, y: RefNode T, z: RefNode T, w: RefNode T :: {Between(f, y, z, w), f[x]} Between(f, x, f[x]->next, f[x]->next));
 
 // reach
-axiom {:ctor "Node"} (forall<T> f: [RefNode T]RefNode T, x: RefNode T, y: RefNode T :: {f[x], Between(f, x, y, y)} Between(f, x, y, y) ==> x == y || Between(f, x, f[x], y));
+axiom {:ctor "Node"} (forall<T> f: [RefNode T]Node T, x: RefNode T, y: RefNode T :: {f[x], Between(f, x, y, y)} Between(f, x, y, y) ==> x == y || Between(f, x, f[x]->next, y));
 
 // cycle
-axiom {:ctor "Node"} (forall<T> f: [RefNode T]RefNode T, x: RefNode T, y:RefNode T :: {f[x], Between(f, x, y, y)} f[x] == x && Between(f, x, y, y) ==> x == y);
+axiom {:ctor "Node"} (forall<T> f: [RefNode T]Node T, x: RefNode T, y:RefNode T :: {f[x], Between(f, x, y, y)} f[x]->next == x && Between(f, x, y, y) ==> x == y);
 
 // sandwich
-axiom {:ctor "Node"} (forall<T> f: [RefNode T]RefNode T, x: RefNode T, y: RefNode T :: {Between(f, x, y, x)} Between(f, x, y, x) ==> x == y);
+axiom {:ctor "Node"} (forall<T> f: [RefNode T]Node T, x: RefNode T, y: RefNode T :: {Between(f, x, y, x)} Between(f, x, y, x) ==> x == y);
 
 // order1
-axiom {:ctor "Node"} (forall<T> f: [RefNode T]RefNode T, x: RefNode T, y: RefNode T, z: RefNode T :: {Between(f, x, y, y), Between(f, x, z, z)} Between(f, x, y, y) && Between(f, x, z, z) ==> Between(f, x, y, z) || Between(f, x, z, y));
+axiom {:ctor "Node"} (forall<T> f: [RefNode T]Node T, x: RefNode T, y: RefNode T, z: RefNode T :: {Between(f, x, y, y), Between(f, x, z, z)} Between(f, x, y, y) && Between(f, x, z, z) ==> Between(f, x, y, z) || Between(f, x, z, y));
 
 // order2
-axiom {:ctor "Node"} (forall<T> f: [RefNode T]RefNode T, x: RefNode T, y: RefNode T, z: RefNode T :: {Between(f, x, y, z)} Between(f, x, y, z) ==> Between(f, x, y, y) && Between(f, y, z, z));
+axiom {:ctor "Node"} (forall<T> f: [RefNode T]Node T, x: RefNode T, y: RefNode T, z: RefNode T :: {Between(f, x, y, z)} Between(f, x, y, z) ==> Between(f, x, y, y) && Between(f, y, z, z));
 
 // transitive1
-axiom {:ctor "Node"} (forall<T> f: [RefNode T]RefNode T, x: RefNode T, y: RefNode T, z: RefNode T :: {Between(f, x, y, y), Between(f, y, z, z)} Between(f, x, y, y) && Between(f, y, z, z) ==> Between(f, x, z, z));
+axiom {:ctor "Node"} (forall<T> f: [RefNode T]Node T, x: RefNode T, y: RefNode T, z: RefNode T :: {Between(f, x, y, y), Between(f, y, z, z)} Between(f, x, y, y) && Between(f, y, z, z) ==> Between(f, x, z, z));
 
 // transitive2
-axiom {:ctor "Node"} (forall<T> f: [RefNode T]RefNode T, x: RefNode T, y: RefNode T, z: RefNode T, w: RefNode T :: {Between(f, x, y, z), Between(f, y, w, z)} Between(f, x, y, z) && Between(f, y, w, z) ==> Between(f, x, y, w) && Between(f, x, w, z));
+axiom {:ctor "Node"} (forall<T> f: [RefNode T]Node T, x: RefNode T, y: RefNode T, z: RefNode T, w: RefNode T :: {Between(f, x, y, z), Between(f, y, w, z)} Between(f, x, y, z) && Between(f, y, w, z) ==> Between(f, x, y, w) && Between(f, x, w, z));
 
 // transitive3
-axiom {:ctor "Node"} (forall<T> f: [RefNode T]RefNode T, x: RefNode T, y: RefNode T, z: RefNode T, w: RefNode T :: {Between(f, x, y, z), Between(f, x, w, y)} Between(f, x, y, z) && Between(f, x, w, y) ==> Between(f, x, w, z) && Between(f, w, y, z));
+axiom {:ctor "Node"} (forall<T> f: [RefNode T]Node T, x: RefNode T, y: RefNode T, z: RefNode T, w: RefNode T :: {Between(f, x, y, z), Between(f, x, w, y)} Between(f, x, y, z) && Between(f, x, w, y) ==> Between(f, x, w, z) && Between(f, w, y, z));
 
 // This axiom is required to deal with the incompleteness of the trigger for the reflexive axiom.
 // It cannot be proved using the rest of the axioms.
-axiom {:ctor "Node"} (forall<T> f: [RefNode T]RefNode T, u:RefNode T, x: RefNode T :: {Between(f, u, x, x)} Between(f, u, x, x) ==> Between(f, u, u, x));
+axiom {:ctor "Node"} (forall<T> f: [RefNode T]Node T, u:RefNode T, x: RefNode T :: {Between(f, u, x, x)} Between(f, u, x, x) ==> Between(f, u, u, x));
 
 // relation between Avoiding and Between
-axiom {:ctor "Node"} (forall<T> f: [RefNode T]RefNode T, x: RefNode T, y: RefNode T, z: RefNode T :: {Avoiding(f, x, y, z)} Avoiding(f, x, y, z) <==> (Between(f, x, y, z) || (Between(f, x, y, y) && !Between(f, x, z, z))));
-axiom {:ctor "Node"} (forall<T> f: [RefNode T]RefNode T, x: RefNode T, y: RefNode T, z: RefNode T :: {Between(f, x, y, z)} Between(f, x, y, z) <==> (Avoiding(f, x, y, z) && Avoiding(f, x, z, z)));
+axiom {:ctor "Node"} (forall<T> f: [RefNode T]Node T, x: RefNode T, y: RefNode T, z: RefNode T :: {Avoiding(f, x, y, z)} Avoiding(f, x, y, z) <==> (Between(f, x, y, z) || (Between(f, x, y, y) && !Between(f, x, z, z))));
+axiom {:ctor "Node"} (forall<T> f: [RefNode T]Node T, x: RefNode T, y: RefNode T, z: RefNode T :: {Between(f, x, y, z)} Between(f, x, y, z) <==> (Avoiding(f, x, y, z) && Avoiding(f, x, z, z)));
 
 // update
-axiom {:ctor "Node"} (forall<T> f: [RefNode T]RefNode T, u: RefNode T, v: RefNode T, x: RefNode T, p: RefNode T, q: RefNode T :: {Avoiding(f[p := q], u, v, x)} Avoiding(f[p := q], u, v, x) <==> ((Avoiding(f, u, v, p) && Avoiding(f, u, v, x)) || (Avoiding(f, u, p, x) && p != x && Avoiding(f, q, v, p) && Avoiding(f, q, v, x))));
+axiom {:ctor "Node"} (forall<T> f: [RefNode T]Node T, u: RefNode T, v: RefNode T, x: RefNode T, p: RefNode T, q: Node T :: {Avoiding(f[p := q], u, v, x)} Avoiding(f[p := q], u, v, x) <==> ((Avoiding(f, u, v, p) && Avoiding(f, u, v, x)) || (Avoiding(f, u, p, x) && p != x && Avoiding(f, q->next, v, p) && Avoiding(f, q->next, v, x))));
 
 function {:inline} Empty<T>(): [RefNode T]bool
 {
